% coding:utf-8

\section{Aufgabe 1}
\subsection{a}
\[ S_{xy} 
= \frac{\sum_{i=1}^{n}(x_i - \overline{x})(y_i - \overline{y})}{n - 1} \]
\[ = \frac{\sum_{i=1}^{n}(x_i \cdot y_i - x_i \cdot \overline{y} - 
\overline{x} \cdot y_i + \overline{x} \cdot \overline{y})}{n - 1} \]
\[ = \frac{\sum_{i=1}^{n}(x_i \cdot y_i)
 - \sum_{i=1}^{n}(x_i \cdot \overline{y})
 - \sum_{i=1}^{n}(\overline{x} \cdot y_i) 
 + \sum_{i=1}^{n}(\overline{x} \cdot \overline{y})}{n-1} \]
\[ = \frac{\sum_{i=1}^{n}(x_i \cdot y_i)
 - \overline{y} \cdot \sum_{i=1}^{n}(x_i)
 - \overline{x} \cdot \sum_{i=1}^{n}(y_i) 
 + n \cdot \overline{x} \cdot \overline{y}}{n-1} \]
\[ = \frac{\sum_{i=1}^{n}(x_i \cdot y_i)
 - \overline{y} \cdot n \cdot \overline{x}
 - \overline{x} \cdot n \cdot \overline{y} 
 + n \cdot \overline{x} \cdot \overline{y}}{n-1} \]
\[ = \frac{\sum_{i=1}^{n}(x_i \cdot y_i)
 - n \cdot \overline{x} \cdot \overline{y}}{n-1} \]

\subsection{b}
\[ r = \frac{S_{xy}}{S_x \cdot S_y} \]
