% coding:utf-8

\section{Aufgabe 2}
\subsection{a}
\[ P(A \cap B) =P(A) \cdot P(B) = \frac{3}{4} \cdot \frac{2}{3} = \frac{1}{2} \]
\begin{venndiagram2sets}
  \fillACapB
\end{venndiagram2sets}
\begin{lstlisting}
\begin{venndiagram2sets}
  \fillACapB
\end{venndiagram2sets}
\end{lstlisting}

\subsection{b}
\[ P(A \cup B) = P(A) + P(B) - P(A \cap B) = 
\frac{3}{4} + \frac{2}{3} - \frac{2}{4} = \frac{11}{12} \]
\begin{venndiagram2sets}
  \fillA \fillB
\end{venndiagram2sets}
\begin{lstlisting}
\begin{venndiagram2sets}
  \fillA \fillB
\end{venndiagram2sets}
\end{lstlisting}

\subsection{c}
\[ P(\overline{A \cap B}) = P(\Omega) - P(A \cap B) = 1 - P(A \cap B) = 
1 - \frac{1}{2} = \frac{1}{2} \]
\begin{venndiagram2sets}
  \fillNotAorB \fillANotB \fillBNotA
\end{venndiagram2sets}
\begin{lstlisting}
\begin{venndiagram2sets}
  \fillNotAorB \fillANotB \fillBNotA
\end{venndiagram2sets}
\end{lstlisting}

\subsection{d}
\[ P(\overline{A \cup B}) = P(\Omega) - P(A \cup B) = 1 - P(A \cup B) = 
1 - \frac{11}{12} = \frac{1}{12} \]
\begin{venndiagram2sets}
  \fillNotAorB
\end{venndiagram2sets}
\begin{lstlisting}
\begin{venndiagram2sets}
  \fillNotAorB
\end{venndiagram2sets}
\end{lstlisting}

\subsection{e}
\[ P(A \cup B) = P(A) + P(B) - 2 \cdot P(A \cap B) = 
\frac{3}{4} + \frac{2}{3} - 2 \cdot \frac{2}{4} = \frac{5}{12} \]
\begin{venndiagram2sets}
  \fillANotB \fillBNotA
\end{venndiagram2sets}
\begin{lstlisting}
\begin{venndiagram2sets}
  \fillANotB \fillBNotA
\end{venndiagram2sets}
\end{lstlisting}
